broken tensor core 2d

src/lib/poly/gemm/Kuiper.Poly.GEMM.TensorCore2D.fst
@@ -1,10 +1,11 @@
-module Kuiper.Poly.GEMM.TensorCore
+module Kuiper.Poly.GEMM.TensorCore2D
 
 #lang-pulse
 
 open Kuiper
 
 #set-options "--z3rlimit 20"
+
 
 open Kuiper.Matrix.Reprs.Type
 open Kuiper.Math { even, odd, even_2x, odd_2x1 }
@@ -30,8 +31,226 @@ open Kuiper.Matrix.Tiling
 open Kuiper.Poly.GEMM.Copy
 open Kuiper.Poly.GEMM.Tiled.Common
 
-// FIXME this says that every thread will own a tile, when in fact
-//  every warp should be owning a tile collectively!!!
+open Pulse.Lib.Array
+
+let array_fragment_pts_to
+  (#et : Type0)
+  (#knd : fragment_kind)
+  (#m #n #k : nat)
+  (#l : fragment_layout)
+  ([@@@mkey] farr: array (fragment et knd m n k l))
+  (ems : seq (value_for et knd m n k))
+  : slprop = 
+    exists* (s: lseq (fragment et knd m n k l) (len ems)).
+      farr |-> s **
+      forall+ (i : natlt (Seq.length s)).
+        (s @! i) |-> (ems @! i)
+
+// inline_for_extraction noextract
+// fn populate_fragments
+//   (#et : Type0)
+//   (#m #n #k : nat)
+//   (#knd : fragment_kind)
+//   (#m #n #k : nat)
+//   (#l : fragment_layout)
+//   (arr: array (fragment et knd m n k l))
+//   (#ems : erased (seq (value_for et knd m n k)))
+//   (gm : gpu_matrix et (dims_for knd m n k)._0 (dims_for knd m n k)._1)
+//   preserves
+//     gpu **
+//     gm |-> Frac f em 
+//   requires 
+//     array_fragment_pts_to arr_frags ems
+//   ensures
+//     exists* ems'. array_fragment_pts_to arr_frags ems'
+// {
+
+// }
+
+#push-options "--debug SMTFail --split_queries always"
+inline_for_extraction noextract
+fn subproducts_tc_2d
+  (#et_ab #et_acc : Type0)
+  {| scalar et_ab, scalar et_acc |}
+  (bm bn bk: szp)
+  (tm : szp{tm /? bm})
+  (tn : szp{tn /? bn})
+  (tk : szp{tk /? bk})
+  (wm : szp{wm * tm /? bm})
+  (wn : szp{wn * tn /? bn})
+  (aFrags : array (fragment et_ab FragA tm tn tk FragLRM))
+  (#emAFrags : erased (lseq (ematrix et_ab tm tk) wm))
+  (bFrags : array (fragment et_ab FragB tm tn tk FragLRM))
+  (#emBFrags : erased (seq (ematrix et_ab tk tn)))
+  (accumFrags : array (fragment et_acc FragAcc tm tn tk FragLAcc))
+  (#emAccumFrags : erased (seq (ematrix et_acc tm tn)))
+  (gA : gpu_matrix et_ab (R.row_major bm bk))
+  (gB : gpu_matrix et_ab (R.row_major bk bn))
+  (#eA : ematrix et_ab bm bk)
+  (#eB : ematrix et_ab bk bn)
+  (#fA #fB : perm)
+  (arow: szlt (bm/(wm*tm)))
+  (bcol : szlt (bn/(wn*tn)))
+  preserves
+    gpu **
+    pure (Seq.length emAFrags == wm /\
+          Seq.length emBFrags == wn /\
+          Seq.length emAccumFrags == wm * wn /\
+          SZ.fits (tm * tn)) **
+    gA |-> Frac fA eA **
+    gB |-> Frac fB eB
+  requires
+    array_fragment_pts_to aFrags emAFrags **
+    array_fragment_pts_to bFrags emBFrags **
+    array_fragment_pts_to accumFrags emAccumFrags
+  ensures
+    exists* emAFrags' emBFrags' emAccumFrags'.
+      array_fragment_pts_to aFrags emAFrags' **
+      array_fragment_pts_to bFrags emBFrags' **
+      array_fragment_pts_to accumFrags emAccumFrags'
+{
+  let mut dotIdx : sz = 0sz;
+  while (SZ.(!dotIdx <^ (bk/^tk)))
+    invariant
+      exists*
+        (vdotIdx : sz{vdotIdx <= bk})
+        (emAFrags : erased (lseq (ematrix et_ab tm tk) wm))
+        (emBFrags : erased (lseq (ematrix et_ab tk tn) wn))
+        (emAccumFrags : erased (lseq (ematrix et_acc tm tn) (wm*wn))).
+          dotIdx |-> vdotIdx **
+          array_fragment_pts_to aFrags emAFrags **
+          array_fragment_pts_to bFrags emBFrags **
+          array_fragment_pts_to accumFrags emAccumFrags
+  {
+    open Pulse.Lib.Array;
+    (* only required because of rewrites_to *)
+    let didx = !dotIdx;
+    // Would like to write this here, but then the loop does not type check. Whye does it want to prove that gA |-> eA?
+    // let tile_for_tc_tiles = gpu_matrix_extract_tile_ro' gA (wm*tm) (SZ.v tk) (SZ.v arow) (SZ.v !dotIdx);
+
+    let mut i0 = 0sz;
+    while (SZ.(!i0 <^ wm))
+      invariant
+        exists*
+          (vi : sz{vi <= wm})
+          (emAFrags : erased (lseq (ematrix et_ab tm tk) wm)).
+            i0 |-> vi **
+            array_fragment_pts_to aFrags emAFrags
+    {
+      // create tile for tensor core tiles that belong to the warp
+      let tile_for_tc_tiles = gpu_matrix_extract_tile_ro' gA (wm*tm) (SZ.v tk) (SZ.v arow) (SZ.v !dotIdx);
+      let a_tile = gpu_matrix_extract_tile_ro' tile_for_tc_tiles (SZ.v tm) (SZ.v tk) (SZ.v !i0) 0;
+      // Expected are only nats, but later on when the tile is used we need to concretize.
+      // In this case wm*tm and 0 must be concretizable which means that either we have to write (SZ.v (wm*^tm)) and (SZ.v 0sz),
+      // which is odd, because a nat is expected, or there must be type classes that can resolve this.
+      assert (rewrites_to a_tile (
+        gpu_matrix_subtile (
+          gpu_matrix_subtile gA (wm*tm) (SZ.v tk) (SZ.v arow) (SZ.v didx))
+          (SZ.v tm) (SZ.v tk) (SZ.v !i0) 0));
+
+      unfold array_fragment_pts_to aFrags;
+      with saFrags. assert aFrags |-> saFrags;
+      let a_frag = aFrags.(!i0);
+      forevery_extract' #(natlt (Seq.length saFrags)) !i0 _;
+
+      mma_loadA a_frag a_tile;
+
+      let vdotIdx = !dotIdx;
+      let vi = !i0;
+
+      Pulse.Lib.Forall.elim_forall
+        // type annotation is required, although it is not required in the RefArray example
+        (fun (i : natlt (Seq.length saFrags)) ->
+            if i = (SZ.v vi)
+            then ((saFrags @! i) |-> (ematrix_subtile (ematrix_subtile eA (wm*tm) tk arow vdotIdx) tm tk vi 0))
+            else ((saFrags @! i) |-> (emAFrags @! i)));
+
+      ambig_trade_elim ();
+
+      // Pulse.Lib.Trade.elim_trade _ (forall+ (x: natlt (Seq.Base.length saFrags)).
+      //     match x = SZ.v vi with
+      //     | true ->
+      //       Seq.Base.index saFrags x |->
+      //       ematrix_subtile (ematrix_subtile eA
+      //             (SZ.v wm * SZ.v tm)
+      //             (SZ.v tk)
+      //             (SZ.v arow)
+      //             (SZ.v vdotIdx))
+      //         (SZ.v tm)
+      //         (SZ.v tk)
+      //         (SZ.v vi)
+      //         0
+      //     | _ -> Seq.Base.index saFrags x |-> Seq.Base.index emAFrags x);
+      admit();
+
+
+
+      i0 := !i0 +^ 1sz;
+    };
+
+  //   let mut i1 = 0sz;
+  //   while (SZ.(!i1 <^ wn))
+  //     invariant
+  //       exists*
+  //         (vi : sz{vi <= wn})
+  //         (cbFrags : erased (lseq (ematrix et_ab tk tn) wn)).
+  //           i1 |-> vi **
+  //           bFrags |-> vbFrags
+  //   {
+  //     let tile_for_tc_tiles = gpu_matrix_extract_tile_ro' gB (SZ.v tk) (wn*tn) (SZ.v !dotIdx) (SZ.v bcol);
+  //     let b_tile = gpu_matrix_extract_tile_ro' tile_for_tc_tiles (SZ.v tk) (SZ.v tn) 0 (SZ.v bcol);
+  //     // only rquired because of rewrites_to
+  //     let i1' = !i1;
+  //     assert (rewrites_to b_tile (
+  //       gpu_matrix_subtile (
+  //         gpu_matrix_subtile gB (SZ.v tk) (wn*tn) (SZ.v didx) (SZ.v bcol))
+  //         (SZ.v tk) (SZ.v tn) 0 (SZ.v i1')
+  //       )
+  //     );
+
+  //     mma_loadB bFrags.(!i1) b_tile;
+
+  //     i1 := !i1 +^ 1sz;
+  //   };
+
+  //   let mut resIdxM = 0sz;
+  //   while (SZ.(!resIdxM <^ tm))
+  //     invariant
+  //       exists*
+  //         (vresIdxM : sz{vresIdxM <= tm})
+  //         (vaccumFrags : erased (lseq (ematrix et_acc tm tn) (wm*wn))).
+  //           resIdxM |-> vresIdxM **
+  //           accumFrags |-> vaccumFrags
+  //   {
+  //     let mut resIdxN = 0sz;
+  //     while (SZ.(!resIdxN <^ tn))
+  //       invariant
+  //         exists*
+  //           (vresIdxN : sz{vresIdxN <= tn})
+  //           (vaccumFrags : erased (lseq (ematrix et_acc tm tn) (wm*wn))).
+  //             resIdxN |-> vresIdxN **
+  //             accumFrags |-> vaccumFrags
+  //     {
+  //       let aFrag = aFrags.(!resIdxM);
+  //       let bFrag = bFrags.(!resIdxN);
+  //       let accFrag = accumFrags.(!resIdxM *^ tn +^ !resIdxN);
+
+  //       // can this assertion be removed?
+  //       let iM = !resIdxM;
+  //       let iN = !resIdxN;
+  //       assert(pure(SZ.fits(iM *^ tn +^ iN)));
+
+  //       mma_sync' aFrag bFrag accFrag;
+  //       resIdxN := !resIdxN +^ 1sz;
+  //     };
+
+  //     resIdxM := !resIdxM +^ 1sz;
+  //   };
+
+  //   dotIdx := !dotIdx +^ 1sz;
+  }
+}
+
 let live_thread_tile
   (#et : Type0) {| scalar et |}
   // Since this is an slprop, I would like to not erase the nat.
@@ -50,7 +269,9 @@ let live_thread_tile
   (tid : natlt (bm/tm * (bn/tn)))
   : slprop
   =
-    live (thread_tile (block_tile gC bm bn bid) tm tn tid)
+    exists* em.
+      gpu_matrix_pts_to
+        (thread_tile (block_tile gC bm bn bid) tm tn tid) em
 
 // TODO look again at why we cannot use nats here instead of sizet
 unfold
@@ -82,9 +303,13 @@ let kpre1
   pure (valid_frag_et_dims et_ab FragB tm tn tk) **
   pure (valid_frag_et_dims et_c FragAcc tm tn tk) **
   pure (valid_frag_et_comb et_ab et_c) **
+  // could be added if it wasn't trivially true
+  // pure (valid_frag_et_comb et et) **
   gA |-> Frac (fA /. (rows/tm * (cols/tn))) eA **
   gB |-> Frac (fB /. (rows/tm * (cols/tn))) eB **
-  live_thread_tile gC bm bn tm tn bid tid
+  // see comment at live_thread_tile for why we explicitly
+  // have to convert (so that the reaveal coercion can kick in)
+  live_thread_tile gC (SZ.v bm) (SZ.v bn) (SZ.v tm) (SZ.v tn) bid tid
 
 unfold
 let kpost1
@@ -110,7 +335,7 @@ let kpost1
   =
   gA |-> Frac (fA /. (rows/tm * (cols/tn))) eA **
   gB |-> Frac (fB /. (rows/tm * (cols/tn))) eB **
-  live_thread_tile gC bm bn tm tn bid tid
+  live_thread_tile gC (SZ.v bm) (SZ.v bn) (SZ.v tm) (SZ.v tn) bid tid
 
 let barrier_p
   (#et : Type0)
@@ -126,8 +351,8 @@ let barrier_p
       (exists* (x : ematrix _ _ _). m1 |-> Frac (1.0R /. nthr) x) **
       (exists* (x : ematrix _ _ _). m2 |-> Frac (1.0R /. nthr) x)
     else
-      live_tile_stride_cells m1 nthr tid **
-      live_tile_stride_cells m2 nthr tid
+      own_tile_stride_cells m1 nthr tid **
+      own_tile_stride_cells m2 nthr tid
 
 let barrier_q
   (#et : Type0)
@@ -218,86 +443,17 @@ let kpost
   exists* (x : seq _). fst (snd sh) |-> Frac (1.0R /. (bm/tm * (bn/tn))) x **
   barrier_tok (R.row_major bm bk) (R.row_major bk bn) (fst sh) (fst (snd sh)) (2 * (shared/bk)) (bm/tm * (bn/tn)) tid
 
-
-inline_for_extraction noextract
-fn subproducts_tc
-  (#et_ab #et_acc : Type0)
-  {| scalar et_ab, scalar et_acc |}
-  (bm bn bk: szp)
-  (tm : szp{tm /? bm})
-  (tn : szp{tn /? bn})
-  (tk : szp{tk /? bk})
-  (aFrag : fragment et_ab FragA tm tn tk FragLRM)
-  (#vaFrag : ematrix et_ab tm tk)
-  (bFrag : fragment et_ab FragB tm tn tk FragLRM)
-  (#vbFrag : ematrix et_ab tk tn)
-  (accumFrag : fragment et_acc FragAcc tm tn tk FragLAcc)
-  (#vaccumFrag : ematrix et_acc tm tn)
-  (gA : gpu_matrix et_ab (R.row_major bm bk))
-  (gB : gpu_matrix et_ab (R.row_major bk bn))
-  (#eA : ematrix et_ab bm bk)
-  (#eB : ematrix et_ab bk bn)
-  (#fA #fB : perm)
-  (arow: szlt (bm/tm))
-  (bcol : szlt (bn/tn))
-  preserves
-    gpu **
-    pure (valid_frag_et_comb et_ab et_acc) **
-    gA |-> Frac fA eA **
-    gB |-> Frac fB eB
-  requires
-    aFrag |-> vaFrag **
-    bFrag |-> vbFrag **
-    accumFrag |-> vaccumFrag
-  ensures
-    exists* vaFrag' vbFrag' vaccumFrag'.
-      aFrag |-> vaFrag' **
-      bFrag |-> vbFrag' **
-      accumFrag |-> vaccumFrag'
-{
-  let mut dotIdx : sz = 0sz;
-  while (SZ.(!dotIdx <^ (bk/^tk)))
-    invariant
-      live aFrag **
-      live bFrag **
-      live accumFrag **
-      live dotIdx
-  {
-    (* only required because of rewrites_to *)
-    let a_tile = gpu_matrix_extract_tile_ro' gA (SZ.v tm) (SZ.v tk) (SZ.v arow) (SZ.v !dotIdx);
-    assert (rewrites_to a_tile (gpu_matrix_subtile gA (SZ.v tm) (SZ.v tk) (SZ.v arow) (SZ.v !dotIdx)));
-
-    let b_tile = gpu_matrix_extract_tile_ro' gB (SZ.v tk) (SZ.v tn) (SZ.v !dotIdx) (SZ.v bcol);
-    assert (rewrites_to b_tile (gpu_matrix_subtile gB (SZ.v tk) (SZ.v tn) (SZ.v !dotIdx) (SZ.v bcol)));
-
-    mma_loadA aFrag a_tile;
-    mma_loadB bFrag b_tile;
-    mma_sync' aFrag bFrag accumFrag;
-
-    with etA.
-      assert (gpu_matrix_pts_to a_tile #fA etA);
-      Pulse.Lib.Trade.elim_trade (a_tile |-> Frac fA etA) (gA |-> Frac fA eA);
-    with etB.
-      assert (gpu_matrix_pts_to b_tile #fB etB);
-      Pulse.Lib.Trade.elim_trade (b_tile |-> Frac fB etB) (gB |-> Frac fB eB);
-
-    dotIdx := !dotIdx +^ 1sz;
-  };
-
-  ()
-}
-
 inline_for_extraction noextract
 fn epilogue
   (#et : Type0) {| scalar et |}
   // (comb : binop et)
 
-  // rows should be an erased nat because not concerete value is required, but
+  // rows should be an erased nat because not concrete value is required, but
   // using erased nats here leads to very confusing reveals when calling mma_store
   //  (maybe due to inferred type class instances?)
   // making it a size because otherwise a nat would be extracted
   (#rows : erased nat)
-  // cols is concretized so using size is more succinct
+  // cols is concretized so using size is fine I think
   (#cols : sz)
   (bm : szp{bm /? rows})
   (bn : szp{bn /? cols})
@@ -310,6 +466,7 @@ fn epilogue
   (tid : szlt (bm/tm * (bn/tn)))
   requires
     gpu **
+    // see comment in live_thread_tile for why SZ.v
     live_thread_tile gC bm bn tm tn bid tid **
     (exists* vaccumFrag.
       accumFrag |-> vaccumFrag)
@@ -323,10 +480,10 @@ fn epilogue
 
   (* Only create a tile in gC and write the accumulator values. In this version the input from gC
      was added by loading the tile into the accumulator before any other computations *)
-  let t_tile = thread_tile (block_tile gC (SZ.v bm) (SZ.v bn) (SZ.v bid))
-    (SZ.v tm) (SZ.v tn) (SZ.v tid);
-  assert (rewrites_to t_tile (thread_tile (block_tile gC (SZ.v bm) (SZ.v bn) (SZ.v bid))
-    (SZ.v tm) (SZ.v tn) (SZ.v tid)));
+  let t_tile = thread_tile (block_tile gC (SZ.v bm) (SZ.v bn) (hide (SZ.v bid)))
+    (SZ.v tm) (SZ.v tn) (hide (SZ.v tid));
+  assert (rewrites_to t_tile (thread_tile (block_tile gC (SZ.v bm) (SZ.v bn) (hide (SZ.v bid)))
+    (SZ.v tm) (SZ.v tn) (hide (SZ.v tid))));
 
   // from looking at the type of mma_store, it is not clear that cols mut be concretizable
   // 1. know that strided_row_major needs concrete sizes
@@ -392,6 +549,7 @@ fn kf
   // assert (rewrites_to slA (R.row_major bm bk));
   // let slB = R.row_major bk bn;
   // assert (rewrites_to slB (R.row_major bk bn));
+
   unfold barrier_tok (R.row_major bm bk) (R.row_major bk bn) sarA sarB 0 (bm/tm * (bn/tn)) tid;
 
   gpu_matrix_abs' (R.row_major bm bk) sarA;
@@ -425,7 +583,6 @@ fn kf
   let mut bkIdx  : sz = 0sz;
   while (SZ.(!bkIdx <^ num_k_tiles))
     invariant
-      // Why can I not use `live` here?
       exists* (vbkIdx : SZ.t{vbkIdx <= num_k_tiles})
         (vaFrag : ematrix et_ab tm tk) (vbFrag : ematrix et_ab tk tn) (vaccumFrag : ematrix et_c tm tn).
         bkIdx |-> vbkIdx **
@@ -434,14 +591,13 @@ fn kf
         accumFrag |-> vaccumFrag **
         (exists* (x : ematrix _ _ _). sA |-> Frac (1.0R /. ((bm/tm*(bn/tn)))) x) **
         (exists* (x : ematrix _ _ _). sB |-> Frac (1.0R /. ((bm/tm*(bn/tn)))) x) **
-        B.barrier_tok (barrier_p sA sB ((bm/tm*(bn/tn)))) (barrier_q sA sB ((bm/tm*(bn/tn)))) (2 * !bkIdx) tid
+        B.barrier_tok (barrier_p sA sB ((bm/tm*(bn/tn)))) (barrier_q sA sB ((bm/tm*(bn/tn)))) (2 * vbkIdx) tid
   {
     (* This assert should not be needed. I don't know what effect it even has. *)
-    assert B.barrier_tok (barrier_p sA sB (bm/tm * (bn/tn))) (barrier_q sA sB (bm/tm * (bn/tn))) (2 * !bkIdx) tid;
-    even_2x !bkIdx;
-    assert pure((2 * !bkIdx % 2 = 0) == true);
-    // binding only required because of rewrite
     let vbkIdx = !bkIdx;
+    assert B.barrier_tok (barrier_p sA sB (bm/tm * (bn/tn))) (barrier_q sA sB (bm/tm * (bn/tn))) (2 * vbkIdx) tid;
+    even_2x vbkIdx;
+    assert pure((2 * vbkIdx % 2 = 0) == true);
     rewrite
         (exists* (x : ematrix _ _ _). sA |-> Frac (1.0R /. (bm/tm * (bn/tn))) x) **
         (exists* (x : ematrix _ _ _). sB |-> Frac (1.0R /. (bm/tm * (bn/tn))) x)
@@ -449,16 +605,16 @@ fn kf
 
     B.barrier_wait ();
     rewrite (barrier_q sA sB (bm/tm * (bn/tn)) (2 * vbkIdx) tid)
-        as live_tile_stride_cells sA (bm/tm * (bn/tn)) tid **
-           live_tile_stride_cells sB (bm/tm * (bn/tn)) tid;
+        as own_tile_stride_cells sA (bm/tm * (bn/tn)) tid **
+           own_tile_stride_cells sB (bm/tm * (bn/tn)) tid;
 
     populate_shmem bm bn bk tm tn sA sB gA gB mrow !bkIdx mcol tid;
 
     assert (B.barrier_tok (barrier_p sA sB (bm/tm * (bn/tn))) (barrier_q sA sB (bm/tm * (bn/tn))) (2 * vbkIdx + 1) tid);
     odd_2x1 vbkIdx;
     assert (pure (odd (2 * vbkIdx + 1)));
-    rewrite live_tile_stride_cells sA (bm/tm * (bn/tn)) tid **
-            live_tile_stride_cells sB (bm/tm * (bn/tn)) tid
+    rewrite own_tile_stride_cells sA (bm/tm * (bn/tn)) tid **
+            own_tile_stride_cells sB (bm/tm * (bn/tn)) tid
          as (barrier_p sA sB (bm/tm * (bn/tn)) (2 * vbkIdx + 1) tid);
 
     B.barrier_wait ();
@@ -761,38 +917,4 @@ fn mmcomb_gpu
     (exists* eC'. gC |-> eC')
 {
   launch_sync (mk_kernel gA gB gC bm bn bk tm tn tk (rows/^bm *^ (cols/^bn)) (bm/^tm *^ (bn/^tn)) ());
-}
-
-fn test
-  (gA : gpu_matrix half (R.row_major 1024sz 1024sz))
-  (#eA : ematrix half 1024sz 1024sz)
-  (gB : gpu_matrix half (R.row_major 1024sz 1024sz))
-  (#eB : ematrix half 1024sz 1024sz)
-  (gC : gpu_matrix float (R.row_major 1024sz 1024sz))
-  (#_ : squash (SZ.fits (1024sz * 1024sz)))
-  (#eC : ematrix float 1024sz 1024sz)
-  (#_ : squash (SZ.fits (32*32 + 32/16*(32/16))))
-  (#_ : squash (SZ.fits (32*32 + 32/16*(32/16))))
-  (#_: squash (SZ.fits (32 * 32) /\ SZ.fits (32 * 32)))
-  (#fA #fB : perm)
-  norewrite
-  preserves
-    cpu **
-    gA |-> Frac fA eA **
-    gB |-> Frac fB eB
-  requires
-    pure (1024sz/32 * (1024sz/32) <= max_blocks) **
-    pure (32/16 * (32/16) <= max_threads) **
-    gC |-> eC
-  ensures
-    (exists* eC'. gC |-> eC')
-{
-  launch_sync (
-    mk_kernel
-      #_ #_ #_ #_ #_ #_ #_
-      #_ #(Kuiper.Matrix.Reprs.crepr_row_major.map _ _) gA #_
-      #_ #(Kuiper.Matrix.Reprs.crepr_row_major.map _ _) gB #_
-      gC
-      32sz 32sz 32sz 16sz 16sz 16sz (1024sz/^32sz *^ (1024sz/^32sz)) (32sz/^16sz *^ (32sz/^16sz)) ()
-  );
 }
